\section{The Change of Coordinate Matrix}
\begin{enumerate}
\item \begin{enumerate}
\item No. It should be $[x_j']_{\beta}$.
\item Yes. This is Theorem 2.22.
\item Yes. This is Theorem 2.23.
\item No. It should be $B=Q^{-1}AQ$.
\item Yes. This is the instant result of the definition of similar and Theorem 2.23.
\end{enumerate}
\item For these problem, just calculate $[I]_{\beta'}^{\beta}$.\begin{enumerate}
\item $\left(\begin{array}{cc}a_1&b_1\\a_2&b_2\end{array}\right).$
\item $\left(\begin{array}{cc}4&1\\2&3\end{array}\right).$
\item $\left(\begin{array}{cc}3&-1\\5&-2\end{array}\right).$
\item $\left(\begin{array}{cc}2&-1\\5&-4\end{array}\right).$
\end{enumerate}
\item \begin{enumerate}
\item $\left(\begin{array}{ccc}a_2&b_2&c_2\\a_1&b_1&c_1\\a_0&b_0&c_0\end{array}\right).$
\item $\left(\begin{array}{ccc}a_0&b_0&c_0\\a_1&b_1&c_1\\a_2&b_2&c_2\end{array}\right).$
\item $\left(\begin{array}{ccc}0&-1&0\\1&0&0\\-3&2&1\end{array}\right).$
\item $\left(\begin{array}{ccc}2&1&1\\3&-2&1\\-1&3&1\end{array}\right).$
\item $\left(\begin{array}{ccc}5&-6&3\\0&4&-1\\3&-1&2\end{array}\right).$
\item $\left(\begin{array}{ccc}-2&1&2\\3&4&1\\-1&5&2\end{array}\right).$
\end{enumerate}
\item We have that 
\[[T]_{\beta}=\left(\begin{array}{cc}2&1\\1&-3\end{array}\right)\]
and
\[[T]_{\beta'}=[I]_{\beta}^{\beta'}[[T]_{\beta}[I]_{\beta'}^{\beta}\]
\[=\left(\begin{array}{cc}2&-1\\-1&1\end{array}\right)\left(\begin{array}{cc}2&1\\1&-3\end{array}\right)\left(\begin{array}{cc}1&1\\1&2\end{array}\right)\]
\[=\left(\begin{array}{cc}8&13\\-5&-9\end{array}\right).\]
\item We have that 
\[[T]_{\beta}=\left(\begin{array}{cc}0&0\\1&0\end{array}\right)\]
and
\[[T]_{\beta'}=[I]_{\beta}^{\beta'}[T]_{\beta}[I]_{\beta'}^{\beta}\]
\[=\left(\begin{array}{cc}\frac{1}{2}&\frac{1}{2}\\\frac{1}{2}&-\frac{1}{2}\end{array}\right)\left(\begin{array}{cc}0&1\\0&0\end{array}\right)\left(\begin{array}{cc}1&1\\1&-1\end{array}\right)\]
\[=\left(\begin{array}{cc}\frac{1}{2}&-\frac{1}{2}\\\frac{1}{2}&-\frac{1}{2}\end{array}\right).\]
\item Let $\alpha $ be the standard basis (of $\mathbb{F}^2$ or $\mathbb{F}^3$). We have that $A=[L_A]_{\alpha}$ and hence $[L_A]_{\beta}=[I]_{\alpha}^{\beta}[L_A]_{\alpha}[I]_{\beta}^{\alpha}$. So now we can calculate $[L_A]_{\beta}$ and $Q=[I]_{\beta}^{\alpha}$ and $Q^{-1}=[I]_{\alpha}^{\beta}$.
\begin{enumerate}
\item $[L_A]_{\beta}=\left(\begin{array}{cc}6&11\\-2&-4\end{array}\right)$ and $Q=\left(\begin{array}{cc}1&1\\1&2\end{array}\right)$.
\item $[L_A]_{\beta}=\left(\begin{array}{cc}3&0\\0&-1\end{array}\right)$ and $Q=\left(\begin{array}{cc}1&1\\1&-1\end{array}\right)$.
\item $[L_A]_{\beta}=\left(\begin{array}{ccc}2&2&2\\-2&-3&-4\\1&1&2\end{array}\right)$ and $Q=\left(\begin{array}{ccc}1&1&1\\1&0&1\\1&1&2\end{array}\right)$.
\item $[L_A]_{\beta}=\left(\begin{array}{ccc}6&0&0\\0&12&0\\0&0&18\end{array}\right)$ and $Q=\left(\begin{array}{ccc}1&1&1\\1&-1&1\\-2&0&1\end{array}\right)$.
\end{enumerate}
\item We may let $\beta $ be the standard basis and $\alpha=\{(1,m),(-m,1)\}$ be another basis for $\mathbb{R}^2$.
\begin{enumerate}
\item We have that $[T]_{\alpha}=\left(\begin{array}{cc}1&0\\0&-1\end{array}\right)$ and $Q^{-1}=[I]_{\alpha}^{\beta}=\left(\begin{array}{cc}1&m\\-m&1\end{array}\right)$. We also can calculate that $Q=[I]_{\beta}^{\alpha}=\left(\begin{array}{cc}\frac{1}{m^2+1}&\frac{m}{m^2+1}\\-\frac{m}{m^2+1}&\frac{1}{m^2+1}\end{array}\right)$. So finally we get 
\[[T]_{\beta}=Q^{-1}[T]_{\alpha}Q=\left(\begin{array}{cc}\frac{1-m^2}{m^2+1}&\frac{2m}{m^2+1}\\\frac{2m}{m^2+1}&\frac{m^2-1}{m^2+1}\end{array}\right).\]
That is, $T(x,y)=(\frac{x+2ym-xm^2}{m^2+1},\frac{-y+2xm+ym^2}{m^2+1})$.
\item Similarly we have that $[T]_{\alpha}=\left(\begin{array}{cc}1&0\\0&0\end{array}\right)$. And with the same $Q$ and $Q^{-1}$ we get 
\[[T]_{\beta}=Q^{-1}[T]_{\alpha}Q=\left(\begin{array}{cc}\frac{1}{m^2+1}&\frac{m}{m^2+1}\\\frac{m}{m^2+1}&\frac{m^2}{m^2+1}\end{array}\right).\]
That is, $T(x,y)=(\frac{x+ym}{m^2+1},\frac{xm+ym^2}{m^2+1})$.
\end{enumerate}
\item This is similar to the proof of Theorem 2.23 since 
\[[T]_{\beta'}^{\gamma'}=[I_W]_{\gamma}^{\gamma'}[T]_{\beta}^{\gamma}[I_V]_{\beta'}^{\beta}=P^{-1}[T]_{\beta}^{\gamma}Q.\]
\item We may denote that $A$ is similar to $B$ by $A\sim B$. First we have $A=I^{-1}AI$ and hence $A\sim A$. Second, if $A\sim B$ we have $A=Q^{-1}BQ$ and $B=(Q^{-1})^{-1}AQ^{-1}$ and hence $B\sim A$. Finally, if $A\sim B$ and $B\sim C$ then we have $A=P^{-1}BP$ and $B=Q^{-1}CQ$. And this means $A=(QP)^{-1}C(QP)$ and hence $A\sim C$. So it's a equivalence relation.
\item If $A$ and $B$ are similar, we have $A=Q^{-1}BQ$ for some invertible matrix $Q$. So we have 
\[\mathrm{tr}(A)=\mathrm{tr}(Q^{-1}BQ)=\mathrm{tr}(QQ^{-1}B)=\mathrm{tr}(B)\]
by  Exercise 2.3.13.
\item \begin{enumerate}
\item This is because 
\[RQ=[I]_{\beta}^{\gamma}[I]_{\alpha}^{\beta}=[I]_{\alpha}^{\gamma}.\]
\item This is because 
\[Q^{-1}=([I]_{\alpha}^{\beta})^{-1}=[I^{-1}]_{\beta}^{\alpha}=[I]_{\beta}^{\alpha}.\]
\end{enumerate}
\item This is the instant result that $A=[L_A]_{\beta}$ and $Q$ defined in the Corollary is actually $[I]_{\gamma}^{\beta}$.
\item Since $Q$ is invertible, we have that $L_Q$ is invertible. We try to check $\beta'$ is an independent set and hence a basis since $V$ has dimension $n$. Suppose that $\sum_{j=1}^n{a_jx_j'}=0$. And it means that 
\[\sum_{j=1}^n{a_j\sum_{i=1}^n{Q_{ij}x_i}}=\sum_{i=1}^n{(\sum_{j=1}^n{a_jQ_{ij}})x_i}=0.\]
Since $\beta $ is a basis, we have that $\sum_{j=1}^n{a_jQ_{ij}}=0$ for all $i$. Actually this is a system of linear equations and can be written as 
\[\left(\begin{array}{cccc}a_1&a_2&\ldots &a_n\end{array}\right)\left(\begin{array}{cccc}Q_{11}&Q_{12}&\cdots &Q_{1n}\\Q_{21}&Q_{22}&\cdots &Q_{2n}\\\vdots &\vdots &\ddots &\vdots \\Q_{n1}&Q_{n2}&\cdots &Q_{nn}\end{array}\right)=vQ=0,\]
where $v=\left(\begin{array}{cccc}a_1&a_2&\ldots &a_n\end{array}\right)$.
But since $Q$ is invertible and so $Q^{-1}$ exist, we can deduce that $v=vQQ^{-1}=0Q^{-1}=0$. So we know that $\beta $ is a basis. And it's easy to see that $Q=[I]_{\beta}^{\beta}$ is the change of coordinate matrix changing $\beta'$-coordinates into $\beta$-coordinates.
\item Let $V=\mathbb{F}^n$, $W=\mathbb{F}^m$, $T=L_A$, $\beta $, and $\gamma $ be the notation defined in the Hint. Let $\beta'$ and $\gamma'$ be the set of column vectors of $Q$ and $P$ respectly. By Exercise 2.5.13 we have that $\beta'$ and $\gamma'$ are bases and $Q=[I]_{\beta'}^{\beta}$, $P=[I]_{\gamma'}^{\gamma}$. Since we have that $[T]_{\beta'}^{\gamma'}=[I]_{\gamma}^{\gamma'}[T]_{\beta}^{\gamma}[I]_{\beta'}^{\beta}$, we have that $B=P^{-1}AQ$.
\end{enumerate}
